opentheory/examples/stream.ml
@@ -4,26 +4,47 @@
 
 logfile "stream-def";;
 
-let (stream_abs_rep,stream_rep_abs) =
+let (snth_stream,stream_snth) =
   let exists = prove (`?(s : num -> A). T`, REWRITE_TAC []) in
   let tybij =
-    new_type_definition
-      "stream" ("mk_stream","dest_stream") exists in
-  CONJ_PAIR (REWRITE_RULE [] tybij);;
+      REWRITE_RULE []
+        (new_type_definition "stream" ("stream","snth") exists) in
+  let th1 = prove
+    (`!(s : A stream). stream (snth s) = s`, REWRITE_TAC [tybij])
+  and th2 = prove
+    (`!(f : num -> A). snth (stream f) = f`, REWRITE_TAC [tybij]) in
+  (th1,th2);;
 
-export_thm stream_abs_rep;;
-export_thm stream_rep_abs;;
-
-let stream_tybij = CONJ stream_abs_rep stream_rep_abs;;
+export_thm snth_stream;;
+export_thm stream_snth;;
 
 let shd_def = new_definition
-  `!s : A stream. shd s = dest_stream s 0`;;
+  `!s : A stream. shd s = snth s 0`;;
 
 export_thm shd_def;;
 
+let sdrop_def = new_definition
+  `!(s : A stream) n. sdrop s n = stream (\m. snth s (m + n))`;;
+
+export_thm sdrop_def;;
+
 let stl_def = new_definition
-  `!s : A stream. stl s = mk_stream (\n. dest_stream s (SUC n))`;;
+  `!s : A stream. stl s = sdrop s 1`;;
 
 export_thm stl_def;;
+
+let scons_def = new_definition
+  `!h (t : A stream).
+     scons h t = stream (\n. if n = 0 then h else snth t (n - 1))`;;
+
+export_thm scons_def;;
+
+let ssplit_def = new_definition
+  `!s : A stream.
+     ssplit s =
+     (stream (\n. snth s (2 * n)),
+      stream (\n. snth s (2 * n + 1)))`;;
+
+export_thm ssplit_def;;
 
 logfile_end ();;
